x86/SeqTable.v
@@ -1,0 +1,38 @@
+(** ** Tables *)
+Require Import NArith Lists.List.
+
+(** ** A table storing a sequence of elements. *)
+
+Module SeqTable.
+
+Definition t (V:Type) := list V.
+
+Section WITHV.
+
+  Context {V:Type}.
+
+  Definition get (i:N) (tbl: t V) := 
+    nth_error tbl (N.to_nat i).
+
+  Fixpoint set_nat (i:nat) (v:V) (tbl: t V) :=
+    match i, tbl with
+    | O, h::l =>
+      Some (v::l)
+    | S i', h::l =>
+      match set_nat i' v l with
+      | None => None
+      | Some l' => Some (h :: l')
+      end
+    | _, _ => None
+    end.
+
+  Definition set (i:N) (v: V) (tbl: t V) :=
+    let i' := (N.to_nat i) in
+    set_nat i' v tbl.
+
+  Definition size (tbl:t V) :=
+    length tbl.
+
+End WITHV.
+
+End SeqTable.
