x86/SymbtableEncode.v
@@ -54,7 +54,7 @@ Definition encode_secindex (i:secindex) :=
       match i with
       | secindex_comm => shn_comm
       | secindex_undef => shn_undef
-      | secindex_normal p => Z.pos p
+      | secindex_normal i => Z.of_N i
       end in
   encode_int 2 v.
 
@@ -62,25 +62,30 @@ Section WITH_STRTAB.
 
 Variable (strtab: strtable).
 
-Definition encode_symbentry (id:ident) (e:symbentry)  : res (list byte) :=
-  match strtab ! id with
-  | None => Error (msg "No string associated with this symbol")
-  | Some si => 
-    let st_name_bytes := encode_int32 si in 
-    let st_value_bytes := encode_int32 (symbentry_value e) in
-    let st_size_bytes := encode_int32 (symbentry_size e) in
-    let st_info_bytes := 
-        bytes_of_int 1 (encode_glob_symb_info (symbentry_type e)) in
-    let st_other_bytes := [Byte.repr 0] in
-    let st_shndx_bytes := encode_secindex (symbentry_secindex e) in
-    OK (st_name_bytes ++ st_value_bytes ++ st_size_bytes ++
-                      st_info_bytes ++ st_other_bytes ++ st_shndx_bytes)
-  end.
+Definition encode_symbentry (e:symbentry)  : res (list byte) :=
+  do name_index <-
+      match (symbentry_id e) with
+      | None => OK 0
+      | Some id => 
+        match strtab ! id with
+        | None => Error [MSG "No string associated with this symbol"; POS id]
+        | Some si => OK si
+        end
+      end;
+  let st_name_bytes := encode_int32 name_index in 
+  let st_value_bytes := encode_int32 (symbentry_value e) in
+  let st_size_bytes := encode_int32 (symbentry_size e) in
+  let st_info_bytes := 
+      bytes_of_int 1 (encode_glob_symb_info (symbentry_type e)) in
+  let st_other_bytes := [Byte.repr 0] in
+  let st_shndx_bytes := encode_secindex (symbentry_secindex e) in
+  OK (st_name_bytes ++ st_value_bytes ++ st_size_bytes ++
+                    st_info_bytes ++ st_other_bytes ++ st_shndx_bytes).
   
 Definition encode_symbtable (t:symbtable) : res (list byte) :=
-  fold_right (fun '(id,e) r => 
+  fold_right (fun e r => 
                 do bytes <- r;
-                do ebytes <- (encode_symbentry id e);
+                do ebytes <- (encode_symbentry e);
                 OK (ebytes ++ bytes))
              (OK []) t.
 
